Invariant is correct, changes needed to EclecticLib.

Fifo/Proofs.v
@@ -8,16 +8,48 @@ Require Import Kami.GallinaModules.AuxLemmas.
 Require Import Kami.GallinaModules.AuxTactics.
 Require Import StdLibKami.RegArray.Proofs.
 
-Lemma MaybeEvalPointwise {k} (e1 e2 : Expr type (SyntaxKind (Maybe k))) :
-  evalExpr (e1 @% "valid")%kami_expr = evalExpr (e2 @% "valid")%kami_expr ->
-  evalExpr (e1 @% "data")%kami_expr = evalExpr (e2 @% "data")%kami_expr ->
-  evalExpr e1 = evalExpr e2.
+Lemma emptyb_true {A : Type} (l : list A) :
+  emptyb l = true <-> l = nil.
 Proof.
-  simpl; intros.
-  apply functional_extensionality_dep; intros.
-  fin_dep_destruct x; auto.
-  fin_dep_destruct y; auto.
-  inv y.
+  red; split; destruct l; intros; auto; discriminate.
+Qed.
+
+Lemma emptyb_false {A : Type} (l : list A) :
+  emptyb l = false <-> exists x, In x l.
+Proof.
+  red; split; destruct l; intros; auto; try discriminate.
+  - exists a; left; reflexivity.
+  - dest; inv H.
+Qed.
+
+Lemma emptyb_true_len {A : Type} (l : list A) :
+  emptyb l = true <-> length l = 0.
+Proof.
+  rewrite length_zero_iff_nil; apply emptyb_true.
+Qed.
+
+Lemma emptyb_false_len {A : Type} (l : list A) :
+  emptyb l = false <-> 0 < length l.
+Proof.
+  rewrite emptyb_false; red; split; intros; dest.
+  - destruct l; [inv H| simpl; lia].
+  - destruct l; [simpl in H; lia| exists a; left; reflexivity].
+Qed.
+
+Lemma hd_error_Some {A : Type} (l : list A) (a : A) :
+  hd_error l = Some a <-> l = a :: tl l.
+Proof.
+  red; split; intros.
+  - destruct l; inv H; reflexivity.
+  - rewrite H; reflexivity.
+Qed.
+
+Lemma hd_error_None {A : Type} (l : list A) :
+  hd_error l = None <-> l = nil.
+Proof.
+  red; split; intros.
+  - destruct l; auto; discriminate.
+  - destruct l; auto; discriminate.
 Qed.
 
 Record FifoCorrect {FParams} (imp spec : @Fifo.Ifc.Ifc FParams) : Type :=
@@ -178,7 +210,13 @@ End Proofs2.
 Section Proofs3.
   
   Context {ifcParams' : Fifo.Ifc.Params}.
-  Variable implParams : Impl.Params.
+  (* Context {raIfcParams' : RegArray.Ifc.Params}. *)
+  
+  Variable pow2 : Nat.pow 2 (Nat.log2_up size) = size.
+  Local Definition implParams : Fifo.Impl.Params := 
+    {|Impl.sizePow2 :=  pow2
+      ; Impl.regArray := RegArray.Spec.spec|}.
+  
   Local Definition fifoImpl := @Fifo.Impl.impl ifcParams' implParams.
   Local Definition fifoSpec := @Fifo.Spec.spec ifcParams'.
 
@@ -240,12 +278,12 @@ Section Proofs3.
         destruct x; simpl; rewrite Hsize1; arithmetizeWord; auto.
       - hyp_consumer; goal_consumer2; eauto.
       - hyp_consumer; goal_consumer1.
-        destruct x; cbn[Spec.getHead emptyb negb]; apply functional_extensionality_dep; intros;
-          fin_dep_destruct x; auto; fin_dep_destruct y; auto.
+        destruct x; cbn[Spec.getHead emptyb negb]; apply functional_extensionality_dep;
+          intros; fin_dep_destruct x; auto; fin_dep_destruct y; auto.
       - hyp_consumer; goal_consumer2.
       - hyp_consumer; goal_consumer1.
-        +  destruct x; cbn[Spec.getHead emptyb negb]; apply functional_extensionality_dep; intros;
-             fin_dep_destruct x; auto; fin_dep_destruct y; auto.
+        +  destruct x; cbn[Spec.getHead emptyb negb]; apply functional_extensionality_dep;
+             intros; fin_dep_destruct x; auto; fin_dep_destruct y; auto.
         + econstructor; eauto; normalize_key_concl.
           destruct x; simpl; auto.
       - hyp_consumer; goal_consumer2.
@@ -264,6 +302,287 @@ Section Proofs3.
 
   Section SizeGT1.
     Variable Hsize1 : size <> 1.
+    Definition listInSpec (len start : nat) (arr : Fin.t size -> type k) :=
+      cutList len (rotateList start (convertToList arr)).
+
+    Record myFifoSpecR (o_i o_s : RegsT) : Prop :=
+    {   
+      implRegs : RegsT;
+      specRegs : RegsT;
+      regArray : RegsT;
+      queueLen : Z;
+      enqVal : word (Fifo.Ifc.lgSize + 1);
+      deqVal : word (Fifo.Ifc.lgSize + 1);
+      arrayVal : Fin.t size -> type k;
+      HqueueLen : queueLen = wordVal _ (enqVal ^- deqVal);
+      Hbound : (queueLen <= Z.of_nat size)%Z;
+      implRegVal : implRegs = [(Fifo.Impl.deqPtrName,
+                                existT _ (SyntaxKind (Bit (Fifo.Ifc.lgSize + 1))) deqVal);
+                              (Fifo.Impl.enqPtrName,
+                               existT _ (SyntaxKind (Bit (Fifo.Ifc.lgSize + 1))) enqVal)];
+      regArrayVal : regArray = [((name ++ ".regArray")%string,
+                                  existT _ (SyntaxKind (Array size k)) arrayVal)];
+      specRegVal : specRegs = [(Spec.listName,
+                                     existT (fullType type) (Fifo.Spec.nlist type)
+                                            (listInSpec (Z.to_nat queueLen) (wordToNat deqVal)
+                                                        arrayVal))];
+      Ho_iCorrect : o_i = implRegs ++ regArray;
+      Ho_sCorrect : o_s = specRegs;
+      Ho_iNoDup' : NoDup (map fst o_i);
+    }.
+
+    Ltac Record_destruct :=
+      match goal with
+      |[ H : myFifoSpecR _ _ |- _] => destruct H
+      end.
+    
+    Goal FifoCorrect fifoImpl fifoSpec.
+      assert (size <> 0) as P.
+      { destruct size; auto. }
+      assert (2 ^ (lgSize + 1) <> 0) as P0.
+      { unfold lgSize; intro P0.
+        rewrite Nat.pow_add_r, pow2 in P0.
+        destruct size; simpl in pow2; try lia.
+        simpl in P0; lia.
+      }
+      rewrite <- Nat.eqb_neq in Hsize1.
+      all : econstructor 1 with (fifoR := myFifoSpecR)
+                                (fifoRegs := [(Fifo.Impl.deqPtrName,
+                                               SyntaxKind (Bit (Fifo.Ifc.lgSize + 1)));
+                                              (Fifo.Impl.enqPtrName,
+                                               SyntaxKind (Bit (Fifo.Ifc.lgSize + 1)));
+                                              (Spec.arrayName,
+                                               (SyntaxKind (Array size k)))]).
+      all : red; unfold fifoImpl, fifoSpec, impl, spec, regArray,
+                 isEmpty, flush, enq, deq, numFree, isFull, first,
+                 Impl.isEmpty, Impl.flush, Impl.enq, Impl.deq, Impl.numFree,
+                 Impl.isFull, Impl.first,
+                 Spec.isEmpty, Spec.flush, Spec.enq, Spec.deq, Spec.numFree,
+                 Spec.isFull, Spec.first.
+      all : try rewrite Hsize1; rewrite Nat.eqb_neq in Hsize1.
+      all : unfold Ifc.read, Ifc.write, regArray, implParams, Spec.spec, Spec.read, Spec.write,
+        Impl.isEmpty, Ifc.size, Ifc.k; intros; try Record_destruct.
+      - hyp_consumer.
+        goal_consumer1; simpl.
+        destruct weq; subst; simpl; symmetry; unfold listInSpec.
+        + rewrite Z.sub_diag, Zmod_0_l, cutList_nil_0; reflexivity.
+        + rewrite emptyb_false_len, cutList_length;
+            [|simpl in *; rewrite rotateLength, <- list_arr_length; lia].
+          specialize (Nat.le_0_l
+                        (Z.to_nat ((wordVal (lgSize + 1) x1
+                                    - wordVal (lgSize + 1) x) mod 2 ^ Z.of_nat (lgSize + 1))))
+            as P1.
+          destruct (le_lt_or_eq _ _ P1); auto.
+          exfalso.
+          apply neq_wordVal in n; apply n.
+          specialize (wordBound _ x) as P2; specialize (wordBound _ x1) as P3.
+          rewrite boundProofZIff in *.
+          simpl in Hbound.
+          symmetry in H0.
+          assert (0 = Z.to_nat 0) as TMP by lia; rewrite TMP in H0; clear TMP.
+          apply Z2Nat.inj in H0; try lia; [|apply Z.mod_pos_bound; lia].
+          apply Znumtheory.Zmod_divide_minus in H0; try lia.
+          rewrite Z.sub_0_r in H0; unfold Z.divide in H0; dest.
+          unfold lgSize in *.
+          rewrite <- Zpow_of_nat, Nat.pow_add_r, pow2, Nat2Z.inj_mul in *; simpl in *.
+          destruct (Z_dec 0 x0) as [[P2 | P2] | P2]; try lia.
+          * apply Zlt_le_succ in P2; simpl in P2; try lia.
+            apply (Z.mul_le_mono_nonneg_r _ _ (Z.of_nat size * 2)) in P2; lia.
+          * apply Z.gt_lt in P2.
+            rewrite Z.lt_le_pred in P2; simpl in P2.
+            apply (Z.mul_le_mono_nonneg_r _ _ (Z.of_nat size * 2)) in P2; lia.
+      - hyp_consumer.
+        goal_consumer2; eauto.
+      - hyp_consumer.
+        goal_consumer1; simpl.
+        destruct weq; simpl; symmetry; unfold listInSpec.
+        + rewrite negb_true_iff, Nat.ltb_ge, cutList_length;
+            [|simpl in *; rewrite rotateLength, <- list_arr_length; lia].
+          destruct (Zle_lt_or_eq _ _ Hbound); simpl in *; try lia.
+          exfalso; rewrite <- e in H0; simpl in H0.
+          rewrite Zplus_mod_idemp_r, Zplus_mod_idemp_l,
+          Zminus_mod_idemp_l, Z.add_simpl_l, Z.mod_small in H0; try lia.
+          unfold lgSize in *.
+          rewrite <- Zpow_of_nat, Nat.pow_add_r, pow2, Nat2Z.inj_mul in *; simpl in *; lia.
+        + rewrite negb_false_iff, Nat.ltb_lt, cutList_length;
+            [|simpl in *; rewrite rotateLength, <- list_arr_length; lia].
+          destruct (Zle_lt_or_eq _ _ Hbound); simpl in *; try lia.
+          exfalso.
+          apply neq_wordVal in n; apply n; simpl.
+          rewrite <- H0, Zplus_mod_idemp_l.
+          repeat rewrite Zplus_mod_idemp_r.
+          rewrite Zplus_minus, (wordBound _ x1); reflexivity.
+      - hyp_consumer.
+        goal_consumer2; eauto.
+      - hyp_consumer.
+        goal_consumer1; simpl; unfold listInSpec; rewrite cutList_length;
+          [|simpl in *; rewrite rotateLength, <- list_arr_length; lia].
+        arithmetizeWord; destruct x, x1; simpl in *.
+        rewrite Zminus_mod_idemp_l.
+        rewrite (Z.mod_small
+                   (Z.of_nat size - (wordVal0 - wordVal) mod 2 ^ Z.of_nat (lgSize + 1))
+                   (2 ^ Z.of_nat (lgSize + 1))).
+        + rewrite Nat2Z.inj_sub, Z2Nat.id; try lia.
+          apply Z.mod_pos_bound.
+          unfold lgSize in *.
+          rewrite <- Zpow_of_nat, Nat.pow_add_r, pow2, Nat2Z.inj_mul in *; simpl in *; lia.
+        + unfold lgSize in *.
+          rewrite <- Zpow_of_nat, Nat.pow_add_r, pow2, Nat2Z.inj_mul in *; simpl in *; try lia.
+          specialize (Z.mod_pos_bound (wordVal0 - wordVal) (Z.of_nat size * 2) ltac:(lia)) as P1;
+            lia.
+      - hyp_consumer.
+        goal_consumer2; eauto.
+      - hyp_consumer.
+        goal_consumer1.
+        apply functional_extensionality_dep.
+        intros; fin_dep_destruct x.
+        + simpl; destruct weq; subst; simpl; symmetry; unfold listInSpec.
+          * rewrite negb_false_iff, Z.sub_diag, Zmod_0_l, cutList_nil_0; reflexivity.
+          * rewrite negb_true_iff, emptyb_false_len, cutList_length;
+              [|simpl in *; rewrite rotateLength, <- list_arr_length; lia].
+            specialize (Nat.le_0_l
+                          (Z.to_nat ((wordVal (lgSize + 1) x10
+                                     - wordVal (lgSize + 1) x6)
+                                       mod 2 ^ Z.of_nat (lgSize + 1)))) as P1.
+            destruct (le_lt_or_eq _ _ P1); auto.
+            exfalso.
+            specialize (wordBound _ x6) as P2; specialize (wordBound _ x10) as P3.
+            rewrite boundProofZIff in *.
+            apply neq_wordVal in n; apply n.
+            unfold lgSize in *.
+            rewrite <- Zpow_of_nat, Nat.pow_add_r, pow2, Nat2Z.inj_mul in *; simpl in *; try lia.
+            assert (0 = Z.to_nat 0) as TMP by auto; rewrite TMP in H1 at 1; clear TMP.
+            apply Z2Nat.inj in H1; [|lia |apply Z.mod_pos_bound; lia ].
+            symmetry in H1.
+            apply Z.mod_divide in H1; try lia; unfold Z.divide in H1; dest.
+            destruct (Z_dec 0 x) as [[P2 | P2] | P2]; try lia.
+            -- apply Zlt_le_succ in P2; simpl in P2; try lia.
+               apply (Z.mul_le_mono_nonneg_r _ _ (Z.of_nat size * 2)) in P2; lia.
+            -- apply Z.gt_lt in P2.
+               rewrite Z.lt_le_pred in P2; simpl in P2.
+               apply (Z.mul_le_mono_nonneg_r _ _ (Z.of_nat size * 2)) in P2; lia.
+        + fin_dep_destruct y; auto; unfold Spec.getHead; simpl; destruct weq; simpl;
+            unfold listInSpec.
+          * rewrite e, Z.sub_diag, Zmod_0_l, cutList_nil_0; reflexivity.
+          * destruct lt_dec.
+            -- simpl in Hbound.
+              admit.
+            -- exfalso.
+               unfold lgSize in *.
+               rewrite <- Zpow_of_nat, pow2 in *.
+               apply n0.
+               specialize (Z.mod_pos_bound
+                             (wordVal (Nat.log2_up size + 1) x6)
+                             (Z.of_nat size)
+                             ltac:(lia)) as P1; lia.
+      - hyp_consumer.
+        goal_consumer2.
+      - hyp_consumer.
+        goal_consumer1.
+        + apply functional_extensionality_dep.
+          intros; fin_dep_destruct x.
+          * simpl.
+            destruct weq; subst; simpl; symmetry; unfold listInSpec.
+            -- rewrite Z.sub_diag, Zmod_0_l, cutList_nil_0; reflexivity.
+            -- rewrite negb_true_iff.
+               rewrite emptyb_false_len, cutList_length;
+                 [|simpl in *; rewrite rotateLength, <- list_arr_length; lia].
+               specialize (Nat.le_0_l
+                             (Z.to_nat ((wordVal (lgSize + 1) x19
+                                         - wordVal (lgSize + 1) x13)
+                                          mod 2 ^ Z.of_nat (lgSize + 1))))
+                 as P1.
+               destruct (le_lt_or_eq _ _ P1); auto.
+               exfalso.
+               apply neq_wordVal in n; apply n.
+               specialize (wordBound _ x13) as P2; specialize (wordBound _ x19) as P3.
+               rewrite boundProofZIff in *.
+               simpl in Hbound.
+               symmetry in H1.
+               assert (0 = Z.to_nat 0) as TMP by lia; rewrite TMP in H1; clear TMP.
+               apply Z2Nat.inj in H1; try lia; [|apply Z.mod_pos_bound; lia].
+               apply Znumtheory.Zmod_divide_minus in H1; try lia.
+               rewrite Z.sub_0_r in H1; unfold Z.divide in H1; dest.
+               unfold lgSize in *.
+               rewrite <- Zpow_of_nat, Nat.pow_add_r, pow2, Nat2Z.inj_mul in *; simpl in *.
+               destruct (Z_dec 0 x) as [[P2 | P2] | P2]; try lia.
+               ++ apply Zlt_le_succ in P2; simpl in P2; try lia.
+                  apply (Z.mul_le_mono_nonneg_r _ _ (Z.of_nat size * 2)) in P2; lia.
+               ++ apply Z.gt_lt in P2.
+                  rewrite Z.lt_le_pred in P2; simpl in P2.
+                  apply (Z.mul_le_mono_nonneg_r _ _ (Z.of_nat size * 2)) in P2; lia.
+          * fin_dep_destruct y; auto; unfold Spec.getHead; simpl; destruct weq; simpl;
+            unfold listInSpec.
+            -- rewrite e, Z.sub_diag, Zmod_0_l, cutList_nil_0; reflexivity.
+            -- destruct lt_dec.
+               ++ admit.
+               ++ exfalso.
+                  unfold lgSize in *.
+                  rewrite <- Zpow_of_nat, pow2 in *.
+                  apply n0.
+                  specialize (Z.mod_pos_bound
+                                (wordVal (Nat.log2_up size + 1) x13)
+                                (Z.of_nat size)
+                                ltac:(lia)) as P1; lia.
+        + admit.
+      - hyp_consumer.
+        goal_consumer2.
+      - hyp_consumer.
+        rewrite <- H0 in *.
+        + goal_consumer1.
+          * simpl.
+            destruct weq; symmetry; unfold listInSpec.
+            -- clear H27 H28.
+               rewrite Nat.ltb_ge, cutList_length;
+                 [|simpl in *; rewrite rotateLength, <- list_arr_length; lia].
+               destruct (Zle_lt_or_eq _ _ Hbound); simpl in *; try lia.
+               exfalso; rewrite <- e in H4; simpl in H4.
+               rewrite Zplus_mod_idemp_r, Zplus_mod_idemp_l,
+               Zminus_mod_idemp_l, Z.add_simpl_l, Z.mod_small in H4; try lia.
+               unfold lgSize in *.
+               rewrite <- Zpow_of_nat, Nat.pow_add_r, pow2, Nat2Z.inj_mul in *; simpl in *; lia.
+            -- clear H27 H28; simpl.
+               rewrite Nat.ltb_lt, cutList_length;
+                 [|simpl in *; rewrite rotateLength, <- list_arr_length; lia].
+               destruct (Zle_lt_or_eq _ _ Hbound); simpl in *; try lia.
+               exfalso.
+               apply neq_wordVal in n; apply n; simpl.
+               rewrite <- H4, Zplus_mod_idemp_l.
+               repeat rewrite Zplus_mod_idemp_r.
+               rewrite Zplus_minus, (wordBound _ x10); reflexivity.
+          * admit.
+        + goal_consumer1.
+          * simpl.
+            destruct weq; symmetry; unfold listInSpec; simpl.
+            -- rewrite Nat.ltb_ge, cutList_length;
+                 [|simpl in *; rewrite rotateLength, <- list_arr_length; lia].
+               destruct (Zle_lt_or_eq _ _ Hbound); simpl in *; try lia.
+               exfalso; rewrite <- e in H0; simpl in H0.
+               rewrite Zplus_mod_idemp_r, Zplus_mod_idemp_l,
+               Zminus_mod_idemp_l, Z.add_simpl_l, Z.mod_small in H0; try lia.
+               unfold lgSize in *.
+               rewrite <- Zpow_of_nat, Nat.pow_add_r, pow2, Nat2Z.inj_mul in *; simpl in *; lia.
+            -- rewrite Nat.ltb_lt, cutList_length;
+                 [|simpl in *; rewrite rotateLength, <- list_arr_length; lia].
+               destruct (Zle_lt_or_eq _ _ Hbound); simpl in *; try lia.
+               exfalso.
+               apply neq_wordVal in n; apply n; simpl.
+               rewrite <- H0, Zplus_mod_idemp_l.
+               repeat rewrite Zplus_mod_idemp_r.
+               rewrite Zplus_minus, (wordBound _ x10); reflexivity.
+          * admit.
+      - hyp_consumer.
+        + goal_consumer2.
+        + goal_consumer2; eauto.
+      - hyp_consumer.
+        goal_consumer2.
+        econstructor 1 with (enqVal := $ 0) (deqVal := $ 0); eauto.
+        + simpl; rewrite Zmod_0_l; lia.
+        + simpl; doUpdRegs_red; reflexivity.
+        + simpl; doUpdRegs_red; unfold listInSpec.
+          rewrite cutList_nil_0; reflexivity.
+        + rewrite doUpdRegs_preserves_keys; normalize_key_concl.
+    Admitted.
     
   End SizeGT1.
 
